adding chkr for lt that takes bindings as well.

context.v
@@ -59,6 +59,15 @@ Definition sstack_val_to_cliteral_w_shift (sv : sstack_val) (shift: N) : option 
   | _ => None
   end.
 
+
+Definition sstack_val_to_cliteral_smap (sv : sstack_val) (maxidx: nat) (bs : sbindings) : option cliteral :=
+  match follow_in_smap sv maxidx bs with
+  | Some (FollowSmapVal (SymBasicVal sv') _ _) => sstack_val_to_cliteral sv'
+  | _ => None
+  end.
+
+
+
 Definition chk_eq_wrt_ctx (ctx: ctx_t) (sv1 sv2: sstack_val) :=
   let imp_chkr := imp_checker_fun (ctx_imp_chkr ctx) in
   let cs := ctx_cs ctx in
@@ -74,6 +83,17 @@ Definition chk_lt_wrt_ctx (ctx: ctx_t) (sv1 sv2: sstack_val) :=
   let cs := ctx_cs ctx in
   let ocl1 := sstack_val_to_cliteral sv1 in
   let ocl2 := sstack_val_to_cliteral sv2 in
+  match ocl1, ocl2 with
+  | Some cl1, Some cl2 => imp_chkr cs  (C_LT cl1 cl2)
+  | _, _ => false
+  end.
+
+
+Definition chk_lt_wrt_ctx_smap (ctx: ctx_t) (sv1 sv2: sstack_val) (maxidx: nat) (bs : sbindings) :=
+  let imp_chkr := imp_checker_fun (ctx_imp_chkr ctx) in
+  let cs := ctx_cs ctx in
+  let ocl1 := sstack_val_to_cliteral_smap sv1 maxidx bs in
+  let ocl2 := sstack_val_to_cliteral_smap sv2 maxidx bs in
   match ocl1, ocl2 with
   | Some cl1, Some cl2 => imp_chkr cs  (C_LT cl1 cl2)
   | _, _ => false
