context_facts.v
@@ -280,6 +280,436 @@ Module ContextFacts.
       apply H_chkr_snd.
   Qed.
 
+    Lemma chk_lt_wrt_ctx_smap_snd:
+    forall ctx sv1 sv2 maxidx sb,
+      chk_lt_wrt_ctx_smap ctx sv1 sv2 maxidx sb = true ->
+      forall model mem strg exts ops,
+        is_model (ctx_cs ctx) model = true ->
+        exists v1 v2,
+          eval_sstack_val sv1 model mem strg exts maxidx sb ops = Some v1 /\
+            eval_sstack_val sv2 model mem strg exts maxidx sb ops = Some v2 /\
+            (wordToN v1 < wordToN v2)%N.
+  Proof.
+    intros ctx sv1 sv2 maxidx sb H_chkr model mem strg exts  ops H_is_model.
+    destruct ctx as [cs [chkr H_chkr_snd]].
+    simpl in H_is_model.
+    
+    destruct sv1 as [val1 | var1 | fvar1 ] eqn:E_sv1;
+      destruct sv2 as [val2 | var2 | fvar2 ] eqn:E_sv2;
+      try discriminate.
+
+    (* val1 = val2 *)
+    + unfold chk_lt_wrt_ctx_smap in H_chkr.
+      unfold sstack_val_to_cliteral_smap in H_chkr.
+      rewrite (follow_smap_V val1 maxidx sb) in H_chkr.
+      rewrite (follow_smap_V val2 maxidx sb) in H_chkr.
+      simpl in H_chkr.
+      
+      pose proof (H_chkr_snd cs (C_LT (C_VAL (wordToN val1)) (C_VAL (wordToN val2))) H_chkr) as H_chkr_snd.
+      unfold is_model in H_is_model.
+      unfold imply in H_chkr_snd.
+      pose proof (H_chkr_snd model H_is_model) as H_chkr_snd.
+      unfold satisfies_single_constraint in H_chkr_snd.
+      unfold cliteral_to_nat in H_chkr_snd.
+
+      pose proof (eval_sstack_val_Val val1 model mem strg exts maxidx sb ops) as H_eval_val1. 
+      pose proof (eval_sstack_val_Val val2 model mem strg exts maxidx sb ops) as H_eval_val2.
+
+
+      rewrite N.ltb_lt in H_chkr_snd.
+      
+      rewrite H_eval_val1.
+      rewrite H_eval_val2.
+
+      exists val1.
+      exists val2.
+      repeat split; try reflexivity.
+
+      apply H_chkr_snd.
+
+    (* val = var *)
+    + unfold chk_lt_wrt_ctx_smap in H_chkr.
+      unfold sstack_val_to_cliteral_smap in H_chkr.
+      rewrite (follow_smap_V val1 maxidx sb) in H_chkr.
+      rewrite (follow_smap_InStackVar var2 maxidx sb) in H_chkr.
+      simpl in H_chkr.
+
+      pose proof (H_chkr_snd cs (C_LT (C_VAL (wordToN val1)) (C_VAR var2)) H_chkr) as H_chkr_snd.
+      unfold is_model in H_is_model.
+      unfold imply in H_chkr_snd.
+      pose proof (H_chkr_snd model H_is_model) as H_chkr_snd.
+      unfold satisfies_single_constraint in H_chkr_snd.
+      unfold cliteral_to_nat in H_chkr_snd.
+
+      pose proof (eval_sstack_val_Val val1 model mem strg exts maxidx sb ops) as H_eval_val1. 
+      pose proof (eval_sstack_val_InVar var2 model mem strg exts maxidx sb ops) as H_eval_var2.
+
+
+      rewrite N.ltb_lt in H_chkr_snd.
+      
+      rewrite H_eval_val1.
+      rewrite H_eval_var2.
+
+      exists val1.
+      exists (model var2).
+      repeat split; try reflexivity.
+
+      apply H_chkr_snd.
+
+    (* val = fvar *)
+      
+    + unfold chk_lt_wrt_ctx_smap in H_chkr.
+      unfold sstack_val_to_cliteral_smap in H_chkr.
+      rewrite (follow_smap_V val1 maxidx sb) in H_chkr.
+      destruct (follow_in_smap (FreshVar fvar2) maxidx sb) eqn:E_follow; try destruct f eqn:E_f; try destruct smv eqn:E_smv; try destruct val eqn:E_val; simpl in H_chkr; try discriminate.
+
+      * pose proof (H_chkr_snd cs (C_LT (C_VAL (wordToN val1)) (C_VAL (wordToN val0))) H_chkr) as H_chkr_snd.
+
+        unfold is_model in H_is_model.
+        unfold imply in H_chkr_snd.
+        pose proof (H_chkr_snd model H_is_model) as H_chkr_snd.
+        unfold satisfies_single_constraint in H_chkr_snd.
+        unfold cliteral_to_nat in H_chkr_snd.
+        
+        pose proof (eval_sstack_val_Val val1 model mem strg exts maxidx sb ops) as H_eval_val1. 
+        pose proof (eval_sstack_val_Val val0 model mem strg exts maxidx sb ops) as H_eval_val0.
+        
+        
+        rewrite N.ltb_lt in H_chkr_snd.
+        
+        rewrite H_eval_val1.
+        
+        unfold eval_sstack_val.
+        unfold eval_sstack_val'.
+        rewrite E_follow.
+        
+        
+        exists val1.
+        exists val0.
+        repeat split; try reflexivity.
+        
+        apply H_chkr_snd.
+        
+      * pose proof (H_chkr_snd cs (C_LT (C_VAL (wordToN val1)) (C_VAR var)) H_chkr) as H_chkr_snd.
+        unfold is_model in H_is_model.
+        unfold imply in H_chkr_snd.
+        pose proof (H_chkr_snd model H_is_model) as H_chkr_snd.
+        unfold satisfies_single_constraint in H_chkr_snd.
+        unfold cliteral_to_nat in H_chkr_snd.
+
+        pose proof (eval_sstack_val_Val val1 model mem strg exts maxidx sb ops) as H_eval_val1.
+        rewrite N.ltb_lt in H_chkr_snd.
+        
+        rewrite H_eval_val1.
+        
+        unfold eval_sstack_val.
+        unfold eval_sstack_val'.
+        rewrite E_follow.
+        
+        
+        exists val1.
+        exists (model var).
+        repeat split; try reflexivity.
+        
+        apply H_chkr_snd.
+
+    (* var = val *)
+    + unfold chk_lt_wrt_ctx_smap in H_chkr.
+      unfold sstack_val_to_cliteral_smap in H_chkr.
+
+      rewrite (follow_smap_V val2 maxidx sb) in H_chkr.
+      rewrite (follow_smap_InStackVar var1 maxidx sb) in H_chkr.
+      simpl in H_chkr.
+      pose proof (H_chkr_snd cs (C_LT (C_VAR var1) (C_VAL (wordToN val2))) H_chkr) as H_chkr_snd.
+      unfold is_model in H_is_model.
+      unfold imply in H_chkr_snd.
+      pose proof (H_chkr_snd model H_is_model) as H_chkr_snd.
+      unfold satisfies_single_constraint in H_chkr_snd.
+      unfold cliteral_to_nat in H_chkr_snd.
+
+      pose proof (eval_sstack_val_InVar var1 model mem strg exts maxidx sb ops) as H_eval_var1.
+      pose proof (eval_sstack_val_Val val2 model mem strg exts maxidx sb ops) as H_eval_val2. 
+
+
+      rewrite N.ltb_lt in H_chkr_snd.
+      
+      rewrite H_eval_var1.
+      rewrite H_eval_val2.
+
+      exists (model var1).
+      exists val2.
+      repeat split; try reflexivity.
+
+      apply H_chkr_snd.
+
+    (* var = var *)
+    + unfold chk_lt_wrt_ctx_smap in H_chkr.
+      unfold sstack_val_to_cliteral_smap in H_chkr.
+      rewrite (follow_smap_InStackVar var1 maxidx sb) in H_chkr.
+      rewrite (follow_smap_InStackVar var2 maxidx sb) in H_chkr.
+      simpl in H_chkr.
+      pose proof (H_chkr_snd cs (C_LT (C_VAR var1) (C_VAR var2)) H_chkr) as H_chkr_snd.
+      unfold is_model in H_is_model.
+      unfold imply in H_chkr_snd.
+      pose proof (H_chkr_snd model H_is_model) as H_chkr_snd.
+      unfold satisfies_single_constraint in H_chkr_snd.
+      unfold cliteral_to_nat in H_chkr_snd.
+
+      pose proof (eval_sstack_val_InVar var1 model mem strg exts maxidx sb ops) as H_eval_var1.
+      pose proof (eval_sstack_val_InVar var2 model mem strg exts maxidx sb ops) as H_eval_var2. 
+
+
+      rewrite N.ltb_lt in H_chkr_snd.
+      
+      rewrite H_eval_var1.
+      rewrite H_eval_var2.
+
+      exists (model var1).
+      exists (model var2).
+      repeat split; try reflexivity.
+
+      apply H_chkr_snd.
+
+    (* var = fvar *)
+    + unfold chk_lt_wrt_ctx_smap in H_chkr.
+      unfold sstack_val_to_cliteral_smap in H_chkr.
+      rewrite (follow_smap_InStackVar var1 maxidx sb) in H_chkr.
+      destruct (follow_in_smap (FreshVar fvar2) maxidx sb) eqn:E_follow; try destruct f eqn:E_f; try destruct smv eqn:E_smv; try destruct val eqn:E_val; simpl in H_chkr; try discriminate.
+
+      * pose proof (H_chkr_snd cs (C_LT (C_VAR var1) (C_VAL (wordToN val0))) H_chkr) as H_chkr_snd.
+        unfold is_model in H_is_model.
+        unfold imply in H_chkr_snd.
+        pose proof (H_chkr_snd model H_is_model) as H_chkr_snd.
+        unfold satisfies_single_constraint in H_chkr_snd.
+        unfold cliteral_to_nat in H_chkr_snd.
+
+        pose proof (eval_sstack_val_InVar var1 model mem strg exts maxidx sb ops) as H_eval_var1.
+        rewrite H_eval_var1.
+        
+        unfold eval_sstack_val.
+        unfold eval_sstack_val'.
+        rewrite E_follow.
+        
+        
+        exists (model var1).
+        exists val0.
+        repeat split; try reflexivity.
+        
+        rewrite N.ltb_lt in H_chkr_snd.
+        apply H_chkr_snd.
+
+      * pose proof (H_chkr_snd cs (C_LT (C_VAR var1) (C_VAR var)) H_chkr) as H_chkr_snd.
+        unfold is_model in H_is_model.
+        unfold imply in H_chkr_snd.
+        pose proof (H_chkr_snd model H_is_model) as H_chkr_snd.
+        unfold satisfies_single_constraint in H_chkr_snd.
+        unfold cliteral_to_nat in H_chkr_snd.
+        rewrite N.ltb_lt in H_chkr_snd.
+
+        pose proof (eval_sstack_val_InVar var1 model mem strg exts maxidx sb ops) as H_eval_var1.
+        rewrite H_eval_var1.
+        
+        unfold eval_sstack_val.
+        unfold eval_sstack_val'.
+        rewrite E_follow.
+        
+        
+        exists (model var1).
+        exists (model var).
+        repeat split; try reflexivity.
+        
+        apply H_chkr_snd.
+
+    (* fvar = val *)
+      
+    + unfold chk_lt_wrt_ctx_smap in H_chkr.
+      unfold sstack_val_to_cliteral_smap in H_chkr.
+      rewrite (follow_smap_V val2 maxidx sb) in H_chkr.
+      destruct (follow_in_smap (FreshVar fvar1) maxidx sb) eqn:E_follow; try destruct f eqn:E_f; try destruct smv eqn:E_smv; try destruct val eqn:E_val; simpl in H_chkr; try discriminate.
+
+      * pose proof (H_chkr_snd cs (C_LT (C_VAL (wordToN val0)) (C_VAL (wordToN val2))) H_chkr) as H_chkr_snd.
+
+        unfold is_model in H_is_model.
+        unfold imply in H_chkr_snd.
+        pose proof (H_chkr_snd model H_is_model) as H_chkr_snd.
+        unfold satisfies_single_constraint in H_chkr_snd.
+        unfold cliteral_to_nat in H_chkr_snd.
+        rewrite N.ltb_lt in H_chkr_snd.
+
+        pose proof (eval_sstack_val_Val val2 model mem strg exts maxidx sb ops) as H_eval_val2.
+        rewrite H_eval_val2.
+        
+        unfold eval_sstack_val.
+        unfold eval_sstack_val'.
+        rewrite E_follow.
+        
+        
+        exists val0.
+        exists val2.
+        repeat split; try reflexivity.
+        
+        apply H_chkr_snd.
+        
+      * pose proof (H_chkr_snd cs (C_LT (C_VAR var) (C_VAL (wordToN val2))) H_chkr) as H_chkr_snd.
+        unfold is_model in H_is_model.
+        unfold imply in H_chkr_snd.
+        pose proof (H_chkr_snd model H_is_model) as H_chkr_snd.
+        unfold satisfies_single_constraint in H_chkr_snd.
+        unfold cliteral_to_nat in H_chkr_snd.
+
+        pose proof (eval_sstack_val_Val val2 model mem strg exts maxidx sb ops) as H_eval_val2.
+        rewrite N.ltb_lt in H_chkr_snd.
+        
+        rewrite H_eval_val2.
+        
+        unfold eval_sstack_val.
+        unfold eval_sstack_val'.
+        rewrite E_follow.
+        
+        
+        exists (model var).
+        exists val2.
+        repeat split; try reflexivity.
+        
+        apply H_chkr_snd.
+
+    (* fvar = var *)
+    + unfold chk_lt_wrt_ctx_smap in H_chkr.
+      unfold sstack_val_to_cliteral_smap in H_chkr.
+      rewrite (follow_smap_InStackVar var2 maxidx sb) in H_chkr.
+      destruct (follow_in_smap (FreshVar fvar1) maxidx sb) eqn:E_follow; try destruct f eqn:E_f; try destruct smv eqn:E_smv; try destruct val eqn:E_val; simpl in H_chkr; try discriminate.
+
+      * pose proof (H_chkr_snd cs (C_LT (C_VAL (wordToN val0)) (C_VAR var2)) H_chkr) as H_chkr_snd.
+        unfold is_model in H_is_model.
+        unfold imply in H_chkr_snd.
+        pose proof (H_chkr_snd model H_is_model) as H_chkr_snd.
+        unfold satisfies_single_constraint in H_chkr_snd.
+        unfold cliteral_to_nat in H_chkr_snd.
+        rewrite N.ltb_lt in H_chkr_snd.
+
+        pose proof (eval_sstack_val_InVar var2 model mem strg exts maxidx sb ops) as H_eval_var2.
+        rewrite H_eval_var2.
+        
+        unfold eval_sstack_val.
+        unfold eval_sstack_val'.
+        rewrite E_follow.
+        
+        
+        exists val0.
+        exists (model var2).
+        repeat split; try reflexivity.
+        
+        apply H_chkr_snd.
+
+      * pose proof (H_chkr_snd cs (C_LT (C_VAR var) (C_VAR var2)) H_chkr) as H_chkr_snd.
+        unfold is_model in H_is_model.
+        unfold imply in H_chkr_snd.
+        pose proof (H_chkr_snd model H_is_model) as H_chkr_snd.
+        unfold satisfies_single_constraint in H_chkr_snd.
+        unfold cliteral_to_nat in H_chkr_snd.
+        rewrite N.ltb_lt in H_chkr_snd.
+
+        pose proof (eval_sstack_val_InVar var2 model mem strg exts maxidx sb ops) as H_eval_var2.
+        rewrite H_eval_var2.
+        
+        unfold eval_sstack_val.
+        unfold eval_sstack_val'.
+        rewrite E_follow.
+        
+        
+        exists (model var).
+        exists (model var2).
+        repeat split; try reflexivity.
+        
+        apply H_chkr_snd.
+        
+    (* fvar = fvar *)
+    + unfold chk_lt_wrt_ctx_smap in H_chkr.
+      unfold sstack_val_to_cliteral_smap in H_chkr.
+
+      destruct (follow_in_smap (FreshVar fvar1) maxidx sb) eqn:E_follow1; try destruct f eqn:E_f; try destruct smv eqn:E_smv; try destruct val eqn:E_val;
+      destruct (follow_in_smap (FreshVar fvar2) maxidx sb) eqn:E_follow2; try destruct f0 eqn:E_f0; try destruct smv0 eqn:E_smv0; try destruct val1 eqn:E_val1; try simpl in H_chkr; try discriminate.
+      
+      * pose proof (H_chkr_snd cs (C_LT (C_VAL (wordToN val0)) (C_VAL (wordToN val2))) H_chkr) as H_chkr_snd.
+        unfold is_model in H_is_model.
+        unfold imply in H_chkr_snd.
+        pose proof (H_chkr_snd model H_is_model) as H_chkr_snd.
+        unfold satisfies_single_constraint in H_chkr_snd.
+        unfold cliteral_to_nat in H_chkr_snd.
+        rewrite N.ltb_lt in H_chkr_snd.
+
+        
+        unfold eval_sstack_val.
+        unfold eval_sstack_val'.
+        rewrite E_follow1.
+        rewrite E_follow2.
+
+        exists val0.
+        exists val2.
+        repeat split; try reflexivity.
+
+        apply H_chkr_snd.
+
+      * pose proof (H_chkr_snd cs (C_LT (C_VAL (wordToN val0)) (C_VAR var)) H_chkr) as H_chkr_snd.
+        unfold is_model in H_is_model.
+        unfold imply in H_chkr_snd.
+        pose proof (H_chkr_snd model H_is_model) as H_chkr_snd.
+        unfold satisfies_single_constraint in H_chkr_snd.
+        unfold cliteral_to_nat in H_chkr_snd.
+        rewrite N.ltb_lt in H_chkr_snd.
+        
+        unfold eval_sstack_val.
+        unfold eval_sstack_val'.
+        rewrite E_follow1.
+        rewrite E_follow2.
+
+        exists val0.
+        exists (model var).
+        repeat split; try reflexivity.
+
+        apply H_chkr_snd.
+
+      * destruct val0 eqn:E_val0; simpl in H_chkr; try discriminate.
+
+        **  pose proof (H_chkr_snd cs (C_LT (C_VAR var) (C_VAL (wordToN val1))) H_chkr) as H_chkr_snd.
+        unfold is_model in H_is_model.
+        unfold imply in H_chkr_snd.
+        pose proof (H_chkr_snd model H_is_model) as H_chkr_snd.
+        unfold satisfies_single_constraint in H_chkr_snd.
+        unfold cliteral_to_nat in H_chkr_snd.
+        rewrite N.ltb_lt in H_chkr_snd.
+        
+        unfold eval_sstack_val.
+        unfold eval_sstack_val'.
+        rewrite E_follow1.
+        rewrite E_follow2.
+
+        exists (model var).
+        exists val1.
+        repeat split; try reflexivity.
+
+        apply H_chkr_snd.
+
+        **  pose proof (H_chkr_snd cs (C_LT (C_VAR var) (C_VAR var0))  H_chkr) as H_chkr_snd.
+        unfold is_model in H_is_model.
+        unfold imply in H_chkr_snd.
+        pose proof (H_chkr_snd model H_is_model) as H_chkr_snd.
+        unfold satisfies_single_constraint in H_chkr_snd.
+        unfold cliteral_to_nat in H_chkr_snd.
+        rewrite N.ltb_lt in H_chkr_snd.
+        
+        unfold eval_sstack_val.
+        unfold eval_sstack_val'.
+        rewrite E_follow1.
+        rewrite E_follow2.
+
+        exists (model var).
+        exists (model var0).
+        repeat split; try reflexivity.
+
+        apply H_chkr_snd.
+  Qed.
+
   Lemma chk_neq_wrt_ctx_snd:
     forall ctx sv1 sv2,
       chk_neq_wrt_ctx ctx sv1 sv2 = true ->
